# Differentiation Continued

## Example 1
Find d/dx( sqrt(x<sup>3</sup>) * (e<sup>x</sup> + 2x) )

d/dx( sqrt(x<sup>3</sup>) * (e<sup>x</sup> + 2x) )

= (e<sup>x</sup> + 2x) * d/dx x<sup>3/2</sup> + x<sup>3/2</sup> * d/dx(e<sup>x</sup> + 2x)

= (e<sup>x</sup> + 2x) * 3/2(x<sup>1/2</sup>) + x<sup>3/2</sup> * (e<sup>x</sup> + 2)

= 3/2(x<sup>1/2</sup>)e<sup>x</sup> + 5x<sup>3/2</sup> + x<sup>2/3</sup>e<sup>x</sup>

## Example 2
Find d/dx (x<sup>3</sup>(x<sup>1/2</sup> + 1))

d/dx (x<sup>3</sup>(x<sup>1/2</sup> + 1))

= d/dx (x<sup>7/2</sup> + x<sup>3</sup>)

= d/dx 7/2x<sup>5/2</sup> + 3x<sup>2</sup>

## Example 3
Find d/dx (1 - x<sup>2</sup>)/(1 + x<sup>2</sup>)

d/dx (1 - x<sup>2</sup>)/(1 + x<sup>2</sup>)

= (d/dx(1 - x<sup>2</sup>)(1 + x<sup>2</sup>) - (1 - x<sup>2</sup>)d/dx(1 + x<sup>2</sup>))/(1 + x<sup>2</sup>)<sup>2</sup>

= -4x/(1 + x<sup>2</sup>)<sup>2</sup>

## Example 4
Find d/dx ((sec x)/(1 + tan x))

d/dx ((sec x)/(1 + tan x))

= d/dx((1/cos(x))/(1 + (sin(x)/cos(x))))

= d/dx(1/(cos x + sin x))

= (sin x - cos x)/(cos x + sin x)<sup>2</sup>
